Const fold fuel, potentially

theories/const.v
@@ -2,6 +2,9 @@ From PangoLang Require Import ir.
 Require Import Coq.Program.Wf.
 Require Import FunInd.
 Require Import Lia.
+Require Import Coq.Program.Tactics.
+
+Import CPS.
 
 (** [in_map l f] is just like [map f l] except that the function carries a proof
     that its argument is an element of [l]. *)
@@ -34,18 +37,10 @@ Proof. lia. Qed.
 Program Fixpoint const_fold (exp: cexp) {measure (depth exp)} : cexp :=
     match exp with
     | cbop op (i64 lhs) (i64 rhs) k =>
-        match op with
-        | mul => const_fold (substitute O (i64 (Int64.mul lhs rhs)) k)
-        | add => const_fold (substitute O (i64 (Int64.add lhs rhs)) k)
-        | sub => const_fold (substitute O (i64 (Int64.sub lhs rhs)) k)
-        | _ => exp
-        end
+        cbop op (i64 lhs) (i64 rhs) (const_fold (substitute O (i64 (bop_eval op lhs rhs)) k))
     | cbop op lhs rhs k => cbop op lhs rhs (const_fold k)
     | cuop op (i64 v) k => 
-        match op with
-        | not => const_fold (substitute O (i64 (Int64.not v)) k)
-        | id => const_fold (substitute O (i64 v) k)
-        end
+        cuop op (i64 v) (const_fold (substitute O (i64 (uop_eval op v)) k))
     | cuop op b k => cuop op b (const_fold k)
     | capp x y => capp x y
     | cfix fns k => cfix (in_map fns (fun (e: {a: string * nat * cexp | In a fns}) => 
@@ -57,28 +52,10 @@ Program Fixpoint const_fold (exp: cexp) {measure (depth exp)} : cexp :=
     | fin => fin
     end.
 Next Obligation.
-rewrite <- subst_preserve_depth with (n := O) (v := i64 (Int64.mul lhs rhs)). auto.
+rewrite <- subst_preserve_depth with (n := O) (v := i64 (bop_eval op lhs rhs)). auto.
 Qed.
 Next Obligation.
-rewrite <- subst_preserve_depth with (n := O) (v := i64 (Int64.add lhs rhs)). auto.
-Qed.
-Next Obligation.
-rewrite <- subst_preserve_depth with (n := O) (v := i64 (Int64.sub lhs rhs)). auto.
-Qed.
-Next Obligation. repeat split. all: discriminate. Qed.
-Next Obligation. repeat split. all: discriminate. Qed.
-Next Obligation. repeat split. all: discriminate. Qed.
-Next Obligation. repeat split. all: discriminate. Qed.
-Next Obligation. repeat split. all: discriminate. Qed.
-Next Obligation. repeat split. all: discriminate. Qed.
-Next Obligation. repeat split. all: discriminate. Qed.
-Next Obligation. repeat split. all: discriminate. Qed.
-Next Obligation. repeat split. all: discriminate. Qed.
-Next Obligation. 
-rewrite <- subst_preserve_depth with (n := O) (v := i64 (Int64.not v)). auto.
-Qed.
-Next Obligation.   
-rewrite <- subst_preserve_depth with (n := O) (v := i64 v). auto.
+rewrite <- subst_preserve_depth with (n := O) (v := i64 (uop_eval op v)). auto.
 Qed.
 Next Obligation. simpl. rewrite Nlt_succ_le. apply Nat.max_le_iff.
     left. apply list_max_in. 
@@ -88,3 +65,60 @@ Next Obligation. simpl. auto with arith. Qed.
 Next Obligation. simpl. rewrite Nlt_succ_le. apply list_max_in. apply List.in_map.
 assumption. 
 Defined.
+
+Definition matches s_1 s_2 := s_1.(tr) = s_2.(tr).
+
+Ltac psimpl f := unfold f; rewrite fix_sub_eq; simpl; fold f.
+
+Fixpoint const_fold_fuel (exp: cexp) (fuel: nat): cexp :=
+    match (fuel, exp) with
+    | (S n, cbop op (i64 lhs) (i64 rhs) k) =>
+        cbop op (i64 lhs) (i64 rhs) (const_fold_fuel (substitute O (i64 (bop_eval op lhs rhs)) k) n)
+    | (S n, cbop op lhs rhs k) => cbop op lhs rhs (const_fold_fuel k n)
+    | (S n, cuop op (i64 v) k) => 
+        cuop op (i64 v) (const_fold_fuel (substitute O (i64 (uop_eval op v)) k) n)
+    | (S n, cuop op b k) => cuop op b (const_fold_fuel k n)
+    | (_, capp x y) => capp x y
+    | (S n, cfix fns k) => cfix (map (fun (e: string * nat * cexp) => 
+                                      let '(a, b, k) := e in 
+                                        (a, b, const_fold_fuel k n)) fns) 
+                    (const_fold_fuel k n)
+    | (S n, csel c branches) => csel c (map (fun br => const_fold_fuel br n) branches)
+    | (S n, ceff op args k) => ceff op args (const_fold_fuel k n)
+    | (_, fin) => fin
+    | (O, x) => x
+    end.
+
+Lemma gt_is_succ: forall n m, n > m -> exists n', n = S n'.
+Proof.
+    intros. inversion H as [ m_1 | m_2 ].
+    - now exists m.
+    - now exists m_2.
+Qed. 
+
+
+
+(* TODO: Is this statement actually proving what we want it to prove? *)
+Theorem const_lock_sim: forall c c' s_1 s_2 s_1' n,
+    matches s_1 s_2 -> small_step c s_1 c' s_1' -> n > depth c ->
+    (exists c_2' s_2', small_step (const_fold_fuel c n) s_2 c_2' s_2' /\ matches s_1' s_2').
+Proof.
+    intros. destruct H0. 
+    all: apply gt_is_succ in H1; destruct H1 as (n' & H'); rewrite H'; eexists;
+    eexists; split; (assumption || simpl; auto).
+    (* Select *)
+    - simpl. apply ssel. destruct H0. split.
+        * now rewrite map_length.
+        * assumption.
+    (* Select case 2 *)
+    - assumption.
+    (* Effect *)
+    - unfold matches. unfold matches in H. now rewrite H.
+Qed.    
+
+(* Theorem const_fold_eq: forall n c, n > depth c -> const_fold_fuel c n = const_fold c.
+Proof.
+    induction n.
+    - intros. inversion H.
+    - intros. simpl. destruct c.
+        +    *)
